\begin{itemize}
    \item General p-norm: $||x||_p = (\sum_{i=1}^{n}|x_i|^p)^{1-p}$
    \item Taylor: $f(a) + \frac{f'(a)}{1!}(x-a)  + \frac{f''(a)}{2!}(x-a)^2 + \mathbb{O}(x^3)$
    \item Power series of exp.: $exp(x) := \sum_{k=0}^{\infty}\frac{x^k}{k!}$
    \item $\sum_{k=0}^\infty (xy)^k = \frac{1}{1-xy}$
    \item Entropy: H(X) = $\mathbb{E}_X\left[-log\mathbb{P}(X=x)\right]$
    \item KL-Divergence: \\$D_{KL}(P||Q)=\sum_{x\in \mathbb{X}}P(x)log\left(\frac{P(x)}{Q(x)}\right) \geq 0$
    \item $1-z \leq exp(-z)$
    \item Cauchy-Schwarz: $|\mathbb{E}\left[X,Y\right]|^2 \leq\mathbb{E}(X^2)\mathbb{E}(Y^2)$
    \item Jensens Inequality: for a convex f(X): \\$f(\mathbb{E}(X))\leq\mathbb{E}(f(X))$
    \item M p.s.d. if $v^T M v \succeq 0$
\end{itemize}
Probability Theory:
\begin{itemize}
    \item Gaussian: $\mathcal{N}(x|\mu,\sigma^2) = \frac{1}{\sqrt{2\pi\sigma^2}}exp(-\frac{1}{2}\frac{(x-\mu)^2}{\sigma^2})$
    \item $\mathcal(N)(\boldsymbol{x|\mu,\Sigma}) = \\\frac{1}{\sqrt{(2\pi)^d|\boldsymbol{\Sigma}|}}exp(-\frac{1}{2}(x - \mu)^T\boldsymbol{\Sigma}^{-1}(x-\mu))$
    \item $X\sim\mathcal{N}(\boldsymbol{\mu,\Sigma}), Y=A + BX \Rightarrow \\Y \sim \mathcal{N}(A + B\boldsymbol{\mu},B\boldsymbol{\Sigma^{-1}}B^T)$
    \item Binomial Distr.: $f(k,j;p) = \\\mathbb{P}(X=x)=\begin{pmatrix}
        n\\k
    \end{pmatrix}p^k(1-p)^{n-k}$
    \item $\mathbb{V}(X) = \mathbb{E}\left[(X-\mathbb{E}(X))^2\right]=\mathbb{E}(X^2) - \left[\mathbb{E}(X)\right]^2$
    \item $\mathbb{V}\left[X + Y\right] = \mathbb{V}\left[X\right] + \mathbb{V}\left[Y\right] + 2 Cov(X,Y)$
    \item $Cov(X,Y) = \mathbb{E}\left[(X-\mathbb{E}(X))(Y-\mathbb{E}(Y))\right]$
    \item $Cov(aX,bY) = abCov(X,Y)$
\end{itemize}
Calculus
\begin{itemize}
    \item $\int uv'dx = uv - \int u'vdx$\hspace{0.3cm}$ \bullet\frac{\partial}{\partial x}\frac{g}{h} = \frac{g'h}{h^2} - \frac{gh'}{h^2}$
    \item $\frac{\partial}{\partial\boldsymbol{ x}}(\boldsymbol{b^TAx})=A^Tb$\hspace{0.3cm}$\bullet \frac{\partial}{\partial\boldsymbol{ x}}(\boldsymbol{b^Tx}) = \frac{\partial}{\partial\boldsymbol{ x}}(\boldsymbol{x^Tb}) = b$
    \item $\frac{\partial}{\partial\boldsymbol{ X}}(\boldsymbol{c^TX^Tb}) = \boldsymbol{bc}^T$ \hspace{0.3cm} $\bullet\frac{\partial}{\partial\boldsymbol{ X}}(\boldsymbol{c^TXb}) = \boldsymbol{cb^T}$
    \item $\frac{\partial}{\partial\boldsymbol{ x}}(\boldsymbol{x^TAx})=(\boldsymbol{A^T +A})x \overset{\text{A sym.}}{=} 2\boldsymbol{Ax}$
    \item $\frac{\partial}{\partial\boldsymbol{ X}}Tr(\boldsymbol{X^TA}) = A$\hspace{0.3cm}$\bullet$ Tr.trick: $\boldsymbol{x^TAx} \overset{\text{inner prod.}}{=}\\
    TR(\boldsymbol{x^TAx}) \overset{\text{cyclic perm.}}{=} Tr(\boldsymbol{xx^TA}) = Tr(\boldsymbol{Axx^T})$
    \item $|X^{-1}|=|X|^{-1}$ \hspace{0.02cm} $\bullet \frac{\partial}{\partial\boldsymbol{ X}}log|x|=x^{-T}$ \hspace{0.02cm} $\bullet \frac{\partial}{\partial x}|x| = \frac{x}{|x|}$
    \item $\frac{\partial}{\partial\boldsymbol{ x}}||x||_2 = \frac{\partial}{\partial\boldsymbol{ x}}(\boldsymbol{x^Tx}) = 2x$
    \item $\frac{\partial}{\partial\boldsymbol{ x}}||\boldsymbol{x-b}||_2 = \frac{\boldsymbol{x-b}}{||\boldsymbol{x-b}||_2}$
    \item $\frac{\partial}{\partial\boldsymbol{ x}} ||x||_1 = sgn(x)$
    \item $\sigma(x) = \frac{1}{1 + exp(-x)} \Rightarrow $
    \item $\nabla \sigma(x) = \sigma(x)(1-\sigma(x)) = \sigma(x)\sigma(-x)$
    \item $tanhx = \frac{2sinhx}{2coshx} = \frac{e^x - e^{-x}}{e^x + e^{-x}}$
    \item $\nabla tanhx = 1 - tanh^2x$
    \item $sin(a\pm b) = sin(a)cos(b) \pm cos(a)sin(b)$
    \item $cos(a\pm b) = cos(a)cos(b) \mp sin(a)sin(b)$
\end{itemize}